

$p(n) =$

Alla  $p(n-j)$ ,  $j=1, 2, \dots, n$  ges

av alla  $p(s)$ ,  $0 \leq s \leq n-1$  som redan har beräknats.

$$p(n) = h[j] + p(n-j),$$

$\vdots$

Alla  $p(3-m)$ ,  $m=1, 2, 3$  ges

$$\textcircled{3} \quad p(3) = h[m] + p(3-m), \text{ av } \textcircled{1}, \textcircled{2} \text{ och } p(0)=0$$

Alla  $p(2-k)$ ,  $k=1, 2$  ges

$$\textcircled{2} \quad p(2) = h[k] + p(2-k), \text{ av } \textcircled{1} \text{ och } p(0)=0$$

$$\textcircled{1} \quad p(1) = h[1], \text{ } h \text{ är given}$$